\documentclass{article}
\usepackage[utf8]{inputenc}
\usepackage{geometry}
\usepackage{amsmath}
\usepackage{physics}
\usepackage{dsfont}
\usepackage{graphicx}

\let\vec\boldsymbol

\geometry{margin = 2.5cm}

\title{Method of lines code}
\author{Alexander Prokopyszyn}
\date{June 2020}

\begin{document}

\maketitle

The equations are given by
\[\pdv{u_x}{t}=v_A^2(x,z)\qty[\nabla_{||}b_x - \pdv{b_{||}}{x}],\]
\[\pdv{u_\perp}{t}=v_A^2(x,z)\qty[\nabla_{||}b_\perp-\nabla_\perp b_{||}],\]
\[\pdv{b_x}{t}=\nabla_{||}u_x,\]
\[\pdv{b_\perp}{t}=\nabla_{||}u_{\perp},\]
\[\pdv{b_{||}}{t}=-\qty[\pdv{u_x}{x}+\nabla_\perp u_{\perp}],\]
where
\[\nabla_\perp = \cos\alpha\pdv{}{y} - \sin\alpha\pdv{}{z},\]
\[\nabla_{||} = \sin\alpha\pdv{}{y} + \cos\alpha\pdv{}{z}.\]
The field perturbations $b_x$, $b_\perp$ and $b_{||}$ are dimensionless as they have been normalised by $B_0$. The background field is given by
\[\vec{B}_0=B_0(\sin\alpha\,\vec{\hat{y}}+\cos\alpha\,\vec{\hat{z}}).\]
We assume the variables are of the form
\[f(x,y,z,t) = f'(x,z)\exp\{i[k_\perp(\cos\alpha\,y - \sin\alpha\,z)+\omega t]\}.\]
Note that
\[\nabla_\perp f(x,y,z,t) = \exp\{i[k_\perp(\cos\alpha\,y - \sin\alpha\,z)+\omega t]\}\qty(ik_\perp - \sin\alpha\pdv{}{z})f',\]
\[\nabla_{||} f(x,y,z,t) = \exp\{i[k_\perp(\cos\alpha\,y - \sin\alpha\,z)+\omega t]\}\cos\alpha\pdv{f'}{z} .\]
Therefore, the above equations can be simplified to
\[\pdv{u_x'}{t}=v_A^2(x,z)\qty[\nabla_{||}'b_x' - \pdv{b_{||}'}{x}],\]
\[\pdv{u_\perp'}{t}=v_A^2(x,z)\qty[\nabla_{||}'b_\perp'-\nabla_\perp' b_{||}'],\]
\[\pdv{b_x'}{t}=\nabla_{||}'u_x',\]
\[\pdv{b_\perp'}{t}=\nabla_{||}'u_{\perp}',\]
\[\pdv{b_{||}'}{t}=-\qty[\pdv{u_x'}{x}+\nabla_\perp' u_{\perp}'],\]
where
\[\nabla_\perp' = \qty(ik_\perp - \sin\alpha\pdv{}{z}),\]
\[\nabla_{||}' = \cos\alpha\pdv{}{z}.\]
From this point on, to keep the notation clear, we drop the ' notation.

The equations can be rearranged to give
\[\pdv[2]{u_x}{t}=v_A^2\qty[\nabla_{||}^2u_x - \pdv{b_{||}}{x}{t}],\]
\[\pdv[2]{u_\perp}{t}=v_A^2\qty[\nabla_{||}^2u_\perp -\nabla_\perp\pdv{b_{||}}{t}],\]
hence,
\[\mathcal{L}u_x = i\omega\pdv{b_{||}}{x}\]
\[\mathcal{L}u_\perp = i\omega \nabla_\perp b_{||},\]
where
\[\mathcal{L} = \nabla_{||}^2 + \frac{\omega^2}{v_A^2(x,z)},\]
Therefore,
\[\boxed{\pdv{u_x}{x} = \qty[i\omega b_{||} + \nabla_\perp u_\perp]},\]
\[\boxed{\pdv{b_{||}}{x} = -\frac{i}{\omega}\mathcal{L}u_x,}\]
\[\boxed{\mathcal{L}u_\perp = i\omega \nabla_\perp b_{||}.}\]

We can solve these equations using the method of lines. We discretize in $z$ giving a set of ODEs where the independent variable is $x$. 

Consider the operator, $\mathcal{L}$, given by
\[\mathcal{L} = \cos^2\alpha\pdv[2]{}{z}+\frac{\omega^2}{v_A^2(x,z)}.\]
Using the following discretizing procedure
\[\pdv{f}{z}\rightarrow\frac{1}{\Delta z}(f^{j+1} - f^{j-1})\]
\[\pdv[2]{f}{z}\rightarrow\frac{1}{\Delta z^2}(f^{j+1} - 2 f^{j} + f^{j-1})\]
the $u_\perp$ equation becomes
\[\frac{\cos^2\alpha}{\Delta z^2}(u_\perp^{j+1} - 2u_\perp^j +u_\perp^{j-1}) + \frac{\omega^2}{v_A^2(x,z_j)}u_\perp^j=i\omega\qty[ik_\perp\, b_{||}^j - \frac{\sin\alpha}{\Delta z}(b_{||}^{j+1} - b_{||}^{j-1})].\]
This can be written as
\[a u_\perp^{j-1} + b_j u_\perp^j - au_\perp^{j+1} = d_j,\]
\[a u_\perp^{-1} + b_0 u_\perp^0 - au_\perp^{1} = d_0,\]
\[a u_\perp^{-2} + b_0 u_\perp^{-1} - au_\perp^{0} = d_{-1},\]
where
\[a = \frac{\cos^2\alpha}{\Delta z^2},\]
\[b_j = \frac{\omega^2}{v_A^2(x,z_j)} - 2a\]
\[d_j = -\omega\qty[k_\perp\,b_{||}^j+i\frac{\sin\alpha}{\Delta z}(b_{||}^{j+1} - b_{||}^{j-1})],\]
\[d_0 = -\omega\qty[k_\perp\,b_{||}^0+i\frac{\sin\alpha}{\Delta z}(b_{||}^{1} - b_{||}^{-1})],\]
\[d_{-1} = -\omega\qty[k_\perp\,b_{||}^{-1}+i\frac{\sin\alpha}{\Delta z}(b_{||}^{0} - b_{||}^{-2})],\]
Written as a matrix equation this becomes
\[A\vec{u}_\perp = \vec{d},\]
where
\[A = \begin{pmatrix}
b_0 & a   & 0 & 0 & ... & a \\
a   & b_1 & a & 0 & ... & 0 \\
0   & a & b_2 & a & ... & 0 \\
... \\
0 & ... & 0 & a & b_{-2} & a      \\ 
a & ... & 0 & 0 & a      & b_{-1} \\ 
\end{pmatrix},\ \vec{u}_\perp = \begin{pmatrix}
u_\perp^0 \\
u_\perp^1 \\
u_\perp^2 \\
... \\
u_\perp^{-2} \\
u_\perp^{-1}
\end{pmatrix},\ \vec{d} = \begin{pmatrix}
d_0 \\
d_1 \\
d_2 \\
... \\
d_{-2} \\
d_{-1}
\end{pmatrix}.\]
Let 
\[A = A' + \vec{u}\vec{v}^T,\]
where
\[\vec{u} = \begin{pmatrix}
-b_1 \\
0 \\
0 \\
... \\
0 \\
a
\end{pmatrix},\ \vec{v} = \begin{pmatrix}
1 \\
0 \\
0 \\
... \\
0 \\
-a/b_1
\end{pmatrix},
\implies \vec{u}\vec{v}^T = 
\begin{pmatrix}
-b_1 & 0 & ... & 0 & a \\
0    & 0 & ... & 0 & 0 \\
0    & 0 & ... & 0 & 0 \\
... \\
0 & 0 & ... & 0 & 0 \\
a & 0 & ... & 0 & -a^2 / b_1  
\end{pmatrix}.\]
Note that $A'$ is a tridiagonal matrix and can be inverted relatively easily. Using the Sherman-Morrison formula, we can calculate $\vec{u}_\perp$ by first solving
\[A'\vec{y} = \vec{d},\]
for $\vec{y}$, then solving
\[A' \vec{q} = \vec{u},\]
for $\vec{q}$ then computing $\vec{u}_\perp$ as
\[\vec{u}_\perp = \vec{y} - \frac{\vec{v}^T\vec{y}}{1+\vec{v}^T\vec{q}}\vec{q}.\]


\end{document}
